\documentclass{article}
\usepackage{amsmath}

\author{Kenneth P. Esler, Jr.}
\title{Hybrid orbital representation}
\date{\today}

\begin{document}
\newcommand{\vr}{\mathbf{r}}
\maketitle
\begin{equation}
\phi(\vr) = \sum_{\ell=0}^{\ell_\text{max}} \sum_{m=-\ell}^\ell Y_\ell^m (\hat{\Omega})
u_{\ell m}(r),
\end{equation}
where $u_{lm}(r)$ are complex radial functions represented in some
radial basis (e.g. splines).

\section{Real Spherical Harmonics}
\renewcommand{\Re}{\rm Re}
\renewcommand{\Im}{\rm Im}
If $\phi(\vr)$ can be written as purely real, we can change the
representation so that
\begin{equation}
\phi(\vr) = \sum_{l=0}^{l_\text{max}} \sum_{m=-\ell}^\ell Y_{\ell m}(\hat{\Omega})
\bar{u}_{lm}(r),
\end{equation}
where $\bar{Y}_\ell^m$ are the {\em real} spherical harmonics defined by
\begin{equation}
Y_{\ell m} = \begin{cases}
Y_\ell^0 & \mbox{if } m=0\\
{1\over 2}\left(Y_\ell^m+(-1)^m \, Y_\ell^{-m}\right) \ = \Re\left[Y_\ell^m\right]
%\sqrt{2} N_{(\ell,m)} P_\ell^m(\cos \theta) \cos m\varphi 
& \mbox{if } m>0 \\
{1\over i 2}\left(Y_\ell^{-m}-(-1)^{m}\, Y_\ell^{m}\right) = \Im\left[Y_\ell^{-m}\right]
%\sqrt{2} N_{(\ell,m)} P_\ell^{-m}(\cos \theta) \sin m\varphi 
&\mbox{if } m<0.
\end{cases}
\end{equation}
We need then to relate $\bar{u}_{\ell m}$ to $u_{\ell m}$.  We which
to express,
\begin{equation}
\Re\left[\phi(\vr)\right] = \sum_{\ell=0}^{\ell_\text{max}} \sum_{m=-\ell}^\ell
\Re\left[Y_\ell^m (\hat{\Omega}) u_{\ell m}(r)\right]
\end{equation}
in terms of $\bar{u}_{\ell m}(r)$ and $Y_{\ell m}$.
\begin{eqnarray}
\Re\left[Y_\ell^m u_{\ell m}\right] & = & \Re\left[Y_\ell^m\right]
\Re\left[u_{\ell m}\right] - \Im\left[Y_\ell^m\right] \Im\left[u_{\ell m}\right]
\end{eqnarray}
For $m>0$,
\begin{equation}
\Re\left[Y_\ell^m\right] = Y_{\ell m} \qquad \text{and} \qquad \Im\left[Y_\ell^m\right] = Y_{\ell\,-m}.
\end{equation}
For $m<0$,
\begin{equation}
\Re\left[Y_\ell^m\right] = (-1)^m Y_{\ell\, -m} \qquad \text and \qquad \Im\left[Y_\ell^m\right] = -(-1)^m Y_{\ell m}.
\end{equation}
Then for $m > 0$,
\begin{eqnarray}
\bar{u}_{\ell m} & = & \Re\left[u_{\ell m}\right] + (-1)^m \Re\left[u_{\ell\,-m}\right] \\
\bar{u}_{\ell\, -m} & = & -\Im\left[u_{\ell m}\right] + (-1)^m \Im\left[u_{\ell\,-m}\right].
\end{eqnarray}





\end{document}
